CC/Typed/CanonicalForm.lean
@@ -1,0 +1,51 @@
+import Mathlib.Data.Fin.Basic
+import CC.Basic
+import CC.CaptureSet
+import CC.Type
+import CC.Context
+import CC.TypeMap
+import CC.Typed
+import CC.Subcapt
+import CC.Subcapt.Basic
+import CC.Subtype.Basic
+import CC.Subtype.Inversion
+import CC.Typed.Inversion
+import CC.Typed.Subst
+
+namespace CC
+
+theorem Typed.cf_fun' :
+  t0 = Term.abs T' t ->
+  T0 = CType.capt C (PType.arr T U) ->
+  Typed Γ t0 Ct T0 ->
+  ∃ C', Typed (Ctx.extend_var Γ T) t C' U := by
+  intro he1 he2 h
+  induction h <;> try (solve | cases he1 | cases he2)
+  case abs h hd ih =>
+    cases he1; cases he2
+    aesop
+  case sub h hsub ih =>
+    cases he1; cases he2
+    cases hsub; rename_i hc hs
+    have h1 := SubtypeP.fun_inv hs
+    cases h1
+    case inl h1 =>
+      cases h1; subst_vars
+      exfalso
+      apply Typed.value_typing <;> (solve | constructor | trivial)
+    case inr h1 =>
+      let ⟨T', U', he, hs1, hs2⟩ := h1
+      clear h1
+      subst_vars
+      have ih' := ih rfl rfl
+      cases ih'; rename_i C0 ih
+      constructor
+      apply Typed.sub
+      apply Typed.narrow_var
+      repeat trivial
+
+theorem Typed.cf_fun :
+  Typed Γ (Term.abs T' t) Ct (CType.capt C (PType.arr T U)) ->
+  ∃ C', Typed (Ctx.extend_var Γ T) t C' U := by
+  intro h
+  apply Typed.cf_fun' <;> trivial
