CC/Typed/Inversion.lean
@@ -1,0 +1,29 @@
+import Mathlib.Data.Fin.Basic
+
+import CC.Basic
+import CC.CaptureSet
+import CC.Type
+import CC.Context
+import CC.TypeMap
+import CC.Typed
+import CC.Subcapt
+import CC.Subcapt.Basic
+import CC.Subtype.Basic
+import CC.Subtype.Inversion
+
+namespace CC
+
+theorem Typed.value_typing
+  (h : Typed Γ t C T)
+  (hval : Value t) :
+  T ≠ CType.capt C0 (PType.tvar X) := by
+  induction h <;> try (solve | cases hval | aesop)
+  case sub =>
+    rename_i ht hsub ih
+    intro he
+    subst_vars
+    cases hsub; rename_i hsub
+    have h1 := SubtypeP.tvar_inv hsub
+    cases h1
+    subst_vars
+    aesop
